src/ecPV.mli
@@ -121,13 +121,13 @@ val lp_write_r :                 lvalue     pvaccess
 val i_write_r  : ?except:Sx.t -> instr      pvaccess
 val is_write_r : ?except:Sx.t -> instr list pvaccess
 val s_write_r  : ?except:Sx.t -> stmt       pvaccess
-val f_write_r  : ?except:Sx.t -> xpath      pvaccess
+val f_write_r  : ?except:Sx.t -> ?local:bool -> xpath      pvaccess
 
 val e_read_r   : expr       pvaccess
 val i_read_r   : instr      pvaccess
 val is_read_r  : instr list pvaccess
 val s_read_r   : stmt       pvaccess
-val f_read_r   : xpath      pvaccess
+val f_read_r   : ?local:bool -> xpath      pvaccess
 
 (* -------------------------------------------------------------------- *)
 type 'a pvaccess0 = env -> 'a -> PV.t
@@ -136,13 +136,13 @@ val lp_write :                 lvalue     pvaccess0
 val i_write  : ?except:Sx.t -> instr      pvaccess0
 val is_write : ?except:Sx.t -> instr list pvaccess0
 val s_write  : ?except:Sx.t -> stmt       pvaccess0
-val f_write  : ?except:Sx.t -> xpath      pvaccess0
+val f_write  : ?except:Sx.t -> ?local:bool -> xpath      pvaccess0
 
 val e_read  : expr       pvaccess0
 val i_read  : instr      pvaccess0
 val is_read : instr list pvaccess0
 val s_read  : stmt       pvaccess0
-val f_read  : xpath      pvaccess0
+val f_read  : ?local:bool -> xpath      pvaccess0
 
 (* -------------------------------------------------------------------- *)
 exception EqObsInError
